Working on completeness of EPP

src/Network.v
@@ -8,6 +8,7 @@ From Stdlib Require Lists.List.
 Import List.ListNotations.
 Open Scope list_scope.
 Require Import Stdlib.Structures.Equalities.
+Import Actor.Map.Tactics.
 
 Module Insn.
     Inductive t :=
@@ -257,8 +258,8 @@ Definition EPP_N (C : Choreography.t) (N : Network.t) : Prop :=
     forall A PA,
         Actor.Map.MapsTo A PA N
         <->
-        Actor.FSet.In A (Choreography.actors C)
-        /\ EPP A C PA.
+        (*Actor.FSet.In A (Choreography.actors C)*)
+        EPP A C PA.
 
 (* Correctness of EPP *)
 
@@ -272,18 +273,492 @@ Admitted.
 
 Require Import Stdlib.Program.Equality.
 
+Lemma actors_subst : forall I B x v,
+  Actor.FSet.Equal
+    (Choreography.Insn.actors (Choreography.Insn.subst B x v I))
+    (Choreography.Insn.actors I).
+Proof.
+  destruct I; intros; Actor.simplify.
+Qed.
 
-Lemma EPP_subst_neq : forall A C P B x v,
+
+Lemma EPP_disjoint_inversion : forall A I C P,
+  EPP A (I :: C) P ->
+  ~ Actor.FSet.In A (Choreography.Insn.actors I) ->
+  EPP A C P.
+Proof.
+Admitted.
+About Actor.Map.FSetProperties.add_iff.
+Hint Rewrite Actor.Map.FSetProperties.add_iff : actor_db.
+
+
+Lemma EPP_subst_neq : forall C A P B x v,
     A <> B ->
     EPP A C P ->
     EPP A (Choreography.subst B x v C) P.
-Admitted.
+Proof.
+  induction C as [ | I C];
+    intros ? ? ? ? ? Hneq H.
+  { inversion H; subst; constructor. }
+  inversion H; subst; clear H; simpl;
+    try (repeat reduce_eq_dec;
+    repeat Var.Map.Tactics.reduce_eq_dec;
+    simpl;
+    constructor; auto; fail).
+
+  apply EPP_disjoint.
+  { rewrite actors_subst; auto. }
+  destruct (Choreography.Insn.rebound_in B x I) eqn:HI; auto.
+Qed.
+
+Lemma EPP_subst_neq_bwd : forall C A P B x v,
+    A <> B ->
+    EPP A (Choreography.subst B x v C) P ->
+    EPP A C P.
+Proof.
+  intros C A P B x v Hneq.
+  revert P.
+  induction C as [ | I C]; 
+    intros P Hepp; simpl; auto.
+  assert (Hdec : Actor.FSet.In A (Choreography.Insn.actors I) 
+        \/ ~ Actor.FSet.In A (Choreography.Insn.actors I)).
+  {
+    destruct I; simpl; Var.simplify.
+  }
+  destruct Hdec as [Hin | Hin].
+  2:{
+    apply EPP_disjoint; auto.
+    simpl in *.
+    apply EPP_disjoint_inversion in Hepp.
+    destruct (Choreography.Insn.rebound_in B x I) eqn:HB; auto.
+    rewrite actors_subst; auto.
+  }
+
+  destruct I as 
+    [A0 v0 B0 | A0 x0 B0 y0 | A0 x0 v0 | A0 x0 v0 | A0 x0 y0 v0];
+    simpl in *.
+  * simpl in Hin. autorewrite with actor_db in Hin.
+    destruct Hin; subst.
+    + (* A = A0 *)
+      inversion Hepp; subst; clear Hepp;
+      simpl in *; Actor.simplify;
+      constructor; auto.
+      Var.simplify.
+    + (* A = B0 *)
+      inversion Hepp; subst; clear Hepp;
+      simpl in *; Actor.simplify;
+      constructor; auto.
+  * simpl in Hin. autorewrite with actor_db in Hin.
+    destruct Hin; subst.
+    + (* A = A0 *)
+      inversion Hepp; subst; clear Hepp;
+      simpl in *; Actor.simplify;
+      constructor; auto.
+      Var.simplify.
+    + (* A = B0 *)
+      inversion Hepp; subst; clear Hepp;
+      simpl in *; Actor.simplify;
+      constructor; auto.
+      Var.simplify.
+  * simpl in Hin. autorewrite with actor_db in Hin. subst.
+  
+      inversion Hepp; subst; clear Hepp;
+      simpl in *; Actor.simplify;
+      constructor; auto.
+  * simpl in Hin. autorewrite with actor_db in Hin. subst.
+  
+      inversion Hepp; subst; clear Hepp;
+      simpl in *; Actor.simplify;
+      constructor; auto.
+  * simpl in Hin. autorewrite with actor_db in Hin. subst.
+  
+      inversion Hepp; subst; clear Hepp;
+      simpl in *; Actor.simplify;
+      constructor; auto.
+Qed. 
+
+
+
+Lemma add_mem_iff : forall x y s,
+  Var.Map.S.mem x (Var.Map.S.add y s)
+  =
+  if Var.eq_dec x y then true else Var.Map.S.mem x s.
+Proof.
+  intros.
+  rewrite Var.Map.MProofs.FSetProperties.add_b.
+  unfold Var.Map.MProofs.FSetProperties.eqb.
+  Var.simplify.
+Qed.
+#[global] Hint Rewrite add_mem_iff : var_db.
+
+
+Lemma subst_not_in_I : forall I A x v,
+  ~ Actor.FSet.In A (Choreography.Insn.actors I) ->
+  Choreography.Insn.subst A x v I = I.
+Proof.
+  destruct I; intros; simpl in *; Actor.simplify.
+Qed.
+Lemma rebound_not_in_I : forall I A x,
+  ~ Actor.FSet.In A (Choreography.Insn.actors I) ->
+  Choreography.Insn.rebound_in A x I = false.
+Proof.
+  destruct I; intros; simpl in *; Actor.simplify.
+Qed.
+
+Lemma singleton_mem_iff : forall x y,
+  Var.Map.S.mem y (Var.Map.S.singleton x)
+  =
+  if Var.eq_dec x y then true else false.
+Proof.
+  intros.
+  rewrite Var.Map.FSetProperties.singleton_b.
+  auto.
+Qed.
+#[global] Hint Rewrite singleton_mem_iff : var_db.
+
+
 
 Lemma EPP_subst_eq : forall A C P x v,
     EPP A C P ->
     EPP A (Choreography.subst A x v C) (Process.subst x v P).
-Admitted.
+Proof.
+  intros ? ? ? ? ? H.
+  induction H; subst; simpl;
+    Actor.simplify;
+    Var.simplify;
+    simpl;
+    try (constructor; auto; fail).
 
+  rewrite subst_not_in_I; auto.
+  rewrite rebound_not_in_I; auto.
+  apply EPP_disjoint; auto.
+Qed.
+
+
+Lemma EPP_subst_eq_bwd : forall A x v C P',
+  EPP A (Choreography.subst A x v C) P' ->
+  exists P, EPP A C P /\ P' = Process.subst x v P.
+Proof.
+  intros A x v C.
+  induction C as [ | I C];
+    intros P' H;
+    simpl in *.
+  {
+    inversion H; subst.
+    exists []. split; auto.
+  }
+    assert (Hdec : Actor.FSet.In A (Choreography.Insn.actors I) 
+        \/ ~ Actor.FSet.In A (Choreography.Insn.actors I)).
+  {
+    destruct I; simpl; Var.simplify.
+  }
+  destruct Hdec as [Hin | Hin].
+  2:{
+    apply EPP_disjoint_inversion in H; auto.
+    2:{ rewrite actors_subst; auto. }
+    rewrite rebound_not_in_I in H; auto.
+    apply IHC in H.
+    destruct H as [P [H ?]]; subst.
+    exists P; split; auto.
+    apply EPP_disjoint; auto.
+  }
+
+  destruct I as 
+    [A0 v0 B0 y0 | A0 x0 B0 y0 | A0 x0 v0 | A0 x0 v0 | A0 x0 y0 v0];
+    simpl in *.
+  * autorewrite with actor_db in Hin.
+    inversion H; subst; clear H.
+
+    + (* A = A0 *)
+      Actor.simplify.
+      edestruct (IHC P) as [P0 [H0 ?]]; eauto; subst.
+      exists (Insn.Send v0 B0 :: P0).
+      split; auto.
+      constructor; auto.
+
+    + (* A = B0 *)
+      Actor.simplify.
+      Var.Map.Tactics.compare x y0.
+      - (* x = y0 *)
+        exists (Insn.Receive x A0 :: P).
+        simpl. Var.simplify.
+        split; auto.
+        constructor; auto.
+      
+      - (* x <> y0 *)
+        edestruct (IHC P) as [P0 [H0 ?]]; eauto; subst.
+        exists (Insn.Receive y0 A0 :: P0).
+        simpl. Var.simplify.
+        split; auto.
+        constructor; auto.
+
+    + (* A <> A0 /\ B <> B0 *)
+      (* contradicts Hin *)
+      simpl in *. Actor.simplify.
+      destruct Hin; subst; contradiction.
+
+  * (* EPR *) 
+    autorewrite with actor_db in Hin.
+    inversion H; subst; clear H.
+
+    + (* A = A0 *)
+      Actor.simplify.
+      Var.Map.Tactics.compare x x0.
+      - (* x = y0 *)
+        exists (Insn.EPR x B0 :: P).
+        simpl in *. Var.simplify.
+        split; auto.
+        constructor; auto.
+
+      - (* x <> x0 *)
+        edestruct (IHC P) as [P0 [H0 ?]]; eauto; subst.
+        exists (Insn.EPR x0 B0 :: P0).
+        simpl in *. Var.simplify.
+        split; auto.
+        constructor; auto.
+
+    + (* A = B0 *)
+      Actor.simplify. simpl in *.
+      Var.Map.Tactics.compare x y0.
+      - (* x = y0 *)
+        exists (Insn.EPR x A0 :: P).
+        simpl. Var.simplify.
+        split; auto.
+        constructor; auto.
+      
+      - (* x <> y0 *)
+        edestruct (IHC P) as [P0 [H0 ?]]; eauto; subst.
+        exists (Insn.EPR y0 A0 :: P0).
+        simpl. Var.simplify.
+        split; auto.
+        constructor; auto.
+
+    + (* A <> A0 /\ B <> B0 *)
+      (* contradicts Hin *)
+      simpl in *. Actor.simplify.
+      destruct Hin; subst; contradiction.
+
+  * (* Let *)
+    autorewrite with actor_db in Hin. subst.
+    Actor.simplify.
+    inversion H; subst; clear H.
+    2:{ simpl in *. Actor.simplify. }
+
+    Var.Map.Tactics.compare x x0.
+    + (* x = x0 *)
+      exists (Insn.Let x v0 :: P).
+      simpl. Var.simplify.
+      split; auto.
+      constructor; auto.
+
+    + (* x <> x0 *)
+      edestruct (IHC P) as [P0 [H0 ?]]; eauto; subst.
+      exists (Insn.Let x0 v0 :: P0).
+      simpl; Var.simplify.
+      split; auto.
+      constructor; auto.
+
+
+  * (* LetBang *)
+    autorewrite with actor_db in Hin. subst.
+    Actor.simplify.
+    inversion H; subst; clear H.
+    2:{ simpl in *. Actor.simplify. }
+
+    Var.Map.Tactics.compare x x0.
+    + (* x = x0 *)
+      exists (Insn.LetBang x v0 :: P).
+      simpl. Var.simplify.
+      split; auto.
+      constructor; auto.
+
+    + (* x <> x0 *)
+      edestruct (IHC P) as [P0 [H0 ?]]; eauto; subst.
+      exists (Insn.LetBang x0 v0 :: P0).
+      simpl; Var.simplify.
+      split; auto.
+      constructor; auto.
+
+  
+  * (* LetPair *)
+    autorewrite with actor_db in Hin. subst.
+    Actor.simplify.
+    inversion H; subst; clear H.
+    2:{ simpl in *. Actor.simplify. }
+
+    Var.Map.Tactics.compare x x0;
+      [ | Var.Map.Tactics.compare x y0 ].
+    + (* x = x0 *)
+      exists (Insn.LetPair x y0 v0 :: P).
+      simpl in *. Var.simplify.
+      split; auto.
+      constructor; auto.
+
+    + (* x = y0 *)
+      exists (Insn.LetPair x0 x v0 :: P).
+      simpl in *. Var.simplify.
+      split; auto.
+      constructor; auto.
+
+    + (* x <> x0 /\ x <> y0 *)
+      edestruct (IHC P) as [P0 [H0 ?]]; eauto; subst.
+      exists (Insn.LetPair x0 y0 v0 :: P0).
+      simpl; Var.simplify.
+      split; auto.
+      constructor; auto.
+Qed.
+
+
+Lemma EPP_subst_iff : forall C D PD A x v,
+    EPP D (Choreography.subst A x v C) PD <->
+    (D = A /\ exists PD0,
+                EPP D C PD0 
+                /\ PD = Process.subst x v PD0)
+    \/
+    (D <> A /\ EPP D C PD).
+Proof.
+  intros.
+  split; intros H.
+  * compare A D.
+    + left. split; auto.
+      apply EPP_subst_eq_bwd; auto.
+    + right. split; auto.
+      eapply EPP_subst_neq_bwd; eauto.
+  * destruct H as [[? [PD0 [HPD0 ?]]] | [? HPD]]; subst.
+    + apply EPP_subst_eq; auto.
+    + apply EPP_subst_neq; auto. 
+Qed.
+
+
+
+
+Definition insn_matches_label (I : Choreography.Insn.t) (l : Label.t) : bool :=
+  match I, l with
+  | Choreography.Insn.Send A _ B _, Label.Send A' _ B'
+  | Choreography.Insn.EPR A _ B _, Label.EPR A' B' =>
+    if Actor.eq_dec A A'
+    then if Actor.eq_dec B B' then true else false
+    else false
+  | Choreography.Insn.Let A _ _, Label.Loc A'
+  | Choreography.Insn.LetBang A _ _, Label.Loc A'
+  | Choreography.Insn.LetPair A _ _ _, Label.Loc A' =>
+    if Actor.eq_dec A A' then true else false
+
+  | _, _ => false
+  end.
+
+(** Return the choreography C' such that C, refs -l-> C', refs'
+  * if such a choreography exists.
+  *)
+Inductive step_label : Choreography.t -> ChorEnv.t nat ->
+                       Label.t ->
+                       Choreography.t  -> Prop :=
+
+| StepSend : forall A v B x C refs A' v' B' C',
+  A = A' ->
+  B = B' ->
+  v = v' ->
+  C' = Choreography.subst B x v C ->
+  step_label  (Choreography.Insn.Send A v B x :: C)
+              refs
+              (Label.Send A' v' B')
+              C'
+
+| StepEPR : forall q1 q2 A x B y C refs A' B' C',
+  A = A' ->
+  B = B' ->
+  q1 = Var.fresh (ChorEnv.find A refs) ->
+  q2 = Var.fresh (Var.Map.add x q1 (ChorEnv.find A refs)) ->
+
+  C' = Choreography.subst A x (Expr.Var q1)
+        (Choreography.subst B y (Expr.Var q2)
+        C) ->
+
+  step_label  (Choreography.Insn.EPR A x B y :: C)
+              refs
+              (Label.EPR A' B')
+              C'
+
+| StepLet :forall A x v C refs A' C',
+  A = A' ->
+  C' = Choreography.subst A x v C ->
+  step_label (Choreography.Insn.Let A x v :: C)
+             refs
+             (Label.Loc A')
+             C'
+
+| StepLetBang : forall A x v' C refs A' C',
+  A = A' ->
+  C' = Choreography.subst A x v' C ->
+  step_label (Choreography.Insn.LetBang A x (Expr.Bang v') :: C)
+             refs
+             (Label.Loc A')
+             C'
+
+| StepLetPair : forall A x1 x2 v1 v2 C refs A' C',
+  A = A' ->
+  C' = Choreography.subst A x1 v1 (Choreography.subst A x2 v2 C) ->
+  step_label (Choreography.Insn.LetPair A x1 x2 (Expr.Pair v1 v2) :: C)
+             refs
+             (Label.Loc A')
+             C'
+
+| StepCons : forall I C refs l C',
+  Actor.FSet.Empty
+    (Actor.FSet.inter (Choreography.Label.actors l)
+                      (Choreography.Insn.actors I)) ->
+  step_label C refs l C' ->
+  step_label (I :: C) refs l (I :: C')
+.
+
+(*
+Fixpoint step_label l (refs : Var.Map.t nat) C :=
+  match C with
+  | [] => []
+  | I0 :: C' =>
+
+    match I0 with
+
+    | Choreography.Insn.Send A v B y =>
+      if insn_matches_label I0 l
+      then Choreography.subst B y v C'
+      else I0 :: step_label l refs C'
+
+    | Choreography.Insn.EPR A x B y =>
+      let q1 := Var.fresh refs in
+      let refs' := Var.Map.add x q1 refs in
+      let q2 := Var.fresh refs' in
+      let refs'' := Var.Map.add y q2 refs' in
+
+      if insn_matches_label I0 l
+      then  Choreography.subst A x (Expr.Var q1)
+            (Choreography.subst B y (Expr.Var q2)
+            C')
+      else I0 :: step_label l refs'' C'
+
+    | Choreography.Insn.Let A x v =>
+      if insn_matches_label I0 l
+      then Choreography.subst A x v C'
+      else I0 :: step_label l refs C'
+
+    | Choreography.Insn.LetBang A x (Expr.Bang v') =>
+      if insn_matches_label I0 l
+      then Choreography.subst A x v' C'
+      else I0 :: step_label l refs C'
+
+    | Choreography.Insn.LetPair A x1 x2 (Expr.Pair v1 v2) =>
+      if insn_matches_label I0 l
+      then Choreography.subst A x1 v1
+          (Choreography.subst A x2 v2 C')
+      else I0 :: step_label l refs C'
+
+    | _ => I0 :: step_label l refs C'
+
+    end
+  end.
+  *)
+
+(*
 (** Return the choreography C' such that C -(Send A v B y)-> C' *)
 Fixpoint step_send A B (C : Choreography.t) : Choreography.t :=
     match C with
@@ -295,154 +770,258 @@ Fixpoint step_send A B (C : Choreography.t) : Choreography.t :=
         end
     | I' :: C' => I' :: step_send A B C'
     end.
+  *)
 
-Lemma step_send_complete : forall C A v y B PA PB,
+  
+Lemma step_send_complete : forall C A v y B PA PB refs cfg C',
     EPP A C (Insn.Send v B :: PA) ->
     EPP B C (Insn.Receive y A :: PB) ->
     Expr.Val v ->
-    forall refs cfg,
-        Choreography.step C refs cfg (Label.Send A v B) (step_send A B C) refs cfg.
+    step_label C refs (Label.Send A v B) C' ->
+    Choreography.step C refs cfg (Label.Send A v B)
+                      C' refs cfg.
 Proof.
-    induction C as [ | I C'];
-        intros A v y B PA PB HEPPA HEPPB Hval refs cfg.
+    induction C as [ | I C];
+        intros A v y B PA PB refs cfg C' HEPPA HEPPB Hval Hstep.
     { contradict HEPPA. simpl; inversion 1. }
-    inversion HEPPA; subst;
-    inversion HEPPB; subst; simpl in *;
+    inversion Hstep; subst; clear Hstep.
+
+    inversion HEPPA; subst; clear HEPPA;
+    inversion HEPPB; subst; clear HEPPB;
+      simpl in *;
       Actor.simplify.
     * (* send *)
       apply Choreography.SendB; auto.
         
-    * destruct I as   [ (*Send*) A0 v0 B0 y0
-                    | (*EPR*)  A0 x0 B0 y0
-                    | (*Let*)  A0 x0 e0
-                    | (*Let!*) A0 x0 e0
-                    | (*LetPair *) A0 x0 y0 e0
-      ].
-      + simpl in *. Actor.simplify.
-        apply Choreography.Delay; auto.
-        2:{
-          simpl.
-          intros z.
-          Actor.simplify.
-          intros [Heq1 Heq2].
-          destruct Heq1; destruct Heq2;
-            subst; try contradiction.
-        }
-        eapply IHC'; eauto. 
-
-      + simpl in *. Actor.simplify.
-        apply Choreography.Delay; auto.
-        2:{
-          simpl.
-          intros z.
-          Actor.simplify.
-          intros [Heq1 Heq2].
-          destruct Heq1; destruct Heq2;
-            subst; try contradiction.
-        }
-        eapply IHC'; eauto.
-      + simpl in *. Actor.simplify.
-        apply Choreography.Delay; auto.
-        2:{
-          simpl.
-          intros z.
-          Actor.simplify.
-          intros [Heq1 Heq2].
-          destruct Heq1; destruct Heq2;
-            subst; try contradiction.
-        }
-        eapply IHC'; eauto.
-      + simpl in *. Actor.simplify.
-        apply Choreography.Delay; auto.
-        2:{
-          simpl.
-          intros z.
-          Actor.simplify.
-          intros [Heq1 Heq2].
-          destruct Heq1; destruct Heq2;
-            subst; try contradiction.
-        }
-        eapply IHC'; eauto. 
-      + simpl in *. Actor.simplify.
-        apply Choreography.Delay; auto.
-        2:{
-          simpl.
-          intros z.
-          Actor.simplify.
-          intros [Heq1 Heq2].
-          destruct Heq1; destruct Heq2;
-            subst; try contradiction.
-        }
-        eapply IHC'; eauto.
+    * apply Choreography.Delay; auto.
+        match goal with
+        | [ H : Actor.FSet.Empty _ |- _ ] =>
+          rename H into Hempty
+        end.
+    (*
+      assert (Hin : ~ (Actor.FSet.In A (Choreography.Insn.actors I)) /\ ~ ).
+      {
+        intros Hin.
+        match goal with
+        | [ H : Actor.FSet.Empty _ |- _ ] =>
+          specialize (H A);
+          simpl in H;
+          Actor.simplify
+        end.
+      }
+        *)
+      apply EPP_disjoint_inversion in HEPPA; auto.
+      2:{
+        specialize (Hempty A);
+        simpl in *;
+        Actor.simplify.
+      }
+      apply EPP_disjoint_inversion in HEPPB; auto.
+      2:{
+        specialize (Hempty B);
+        simpl in *;
+        Actor.simplify.
+      }
+      eapply IHC; eauto.
 Qed.
 
-Lemma step_send_EPP_A : forall C A B PA PB v y,
-    EPP A C (Insn.Send v B :: PA) ->
-    EPP B C (Insn.Receive y A :: PB) ->
-    EPP A (step_send A B C) PA.
+
+Lemma EPP_deterministic : forall C A P1 P2,
+  EPP A C P1 ->
+  EPP A C P2 ->
+  P1 = P2.
 Proof.
-  intros C. induction C as [ | I C];
-    intros ? ? ? ? ? ? HA HB;
-    simpl.
-  { inversion HA. }
-  inversion HA; subst; clear HA;
-    simpl; Actor.simplify.
-  { apply EPP_subst_neq; auto. }
-  inversion HB; subst; clear HB;
-    simpl in *; Actor.simplify.
-  destruct I;
-    try (
-        apply EPP_disjoint; auto;
-        eapply IHC; eauto;
-        fail
-    ).
-  simpl in *.
-  Actor.simplify.
-  apply EPP_disjoint; simpl; Actor.simplify.
-  eapply IHC; eauto.
+  induction C as [ | I C]; intros A P1 P2 H1 H2.
+  * inversion H1; inversion H2; subst; clear H1 H2.
+    auto.
+  * inversion H1; inversion H2; subst; clear H1 H2; auto;
+    try discriminate;
+    repeat match goal with
+    | [ H : ?A <> ?A |- _ ] => contradiction
+    | [ H : ?C _ = ?C _ |- _ ] => inversion H; subst; clear H
+    | [ H : ?C _ _ = ?C _ _ |- _ ] => inversion H; subst; clear H
+    | [ H : ?C _ _ _ = ?C _ _ _ |- _ ] => inversion H; subst; clear H
+    | [ H : ?C _ _ _ _ = ?C _ _ _ _ |- _ ] => inversion H; subst; clear H
+    end;
+    f_equal; eauto;
+    simpl in *; Actor.simplify. 
 Qed.
 
-Lemma step_send_EPP_B : forall C A B PA PB v y,
-    EPP A C (Insn.Send v B :: PA) ->
-    EPP B C (Insn.Receive y A :: PB) ->
-    EPP B (step_send A B C) (Process.subst y v PB).
+Lemma EPP_disjoint_iff : forall A I C P,
+  ~ Actor.FSet.In A (Choreography.Insn.actors I) ->
+  EPP A (I :: C) P <-> EPP A C P.
 Proof.
-  intros C. induction C as [ | I C];
-    intros ? ? ? ? ? ? HA HB;
-    simpl.
-  { inversion HB. }
-
-  inversion HA; subst; clear HA;
-  inversion HB; subst; clear HB;
-    simpl in *; Actor.simplify.
-  { apply EPP_subst_eq; auto. }
-
-  destruct I;
-    try (
-      apply EPP_disjoint; auto;
-      simpl in *; Var.simplify;
-      eapply IHC; eauto;
-        fail
-    ).
-    
-  simpl in *.
-  Actor.simplify.
-  apply EPP_disjoint; simpl; Actor.simplify.
-  eapply IHC; eauto.
+  intros. split; intros Hepp.
+  { apply EPP_disjoint_inversion in Hepp; auto. }
+  { apply EPP_disjoint; auto. }
 Qed.
 
-
-Lemma actors_subst : forall A x v I,
-  Actor.FSet.Equal
-    (Choreography.Insn.actors (Choreography.Insn.subst A x v I))
-    (Choreography.Insn.actors I).
+Lemma EPP_cons_iff : forall A I C1 C2,
+  (forall P, EPP A C1 P <-> EPP A C2 P) ->
+  (forall P, EPP A (I :: C1) P <-> EPP A (I :: C2) P).
 Proof.
-  intros; destruct I
-    as [ B1 ?e B2 ?x | B1 ?x B2 ?y | B ?x ?e 
-       | B ?x ?e | B ?x1 ?x2 ?e]; simpl in *;
-    reflexivity.
-Qed.
+  intros A I C1 C2 H P.
   
+Admitted.
+
+Lemma step_label_neq : forall refs l D C C' PD,
+      step_label C refs l C' ->
+      ~ Actor.FSet.In D (Label.actors l) ->
+      EPP D C' PD <-> EPP D C PD.
+Proof.
+  intros ? ? ? ? ? ? Hstep.
+  revert D PD.
+  induction Hstep; intros D PD;
+    subst; simpl; intros Hin; Actor.simplify.
+  * rewrite EPP_disjoint_iff; auto.
+    2:{ simpl; Actor.simplify. }
+    rewrite EPP_subst_iff.
+    intuition.
+
+  * remember (Var.fresh (ChorEnv.find A' refs)) as q1.
+    remember (Var.fresh (Var.Map.add x q1 (ChorEnv.find A' refs))) as q2.
+  
+    rewrite EPP_disjoint_iff; auto.
+    2:{ simpl; Actor.simplify. }
+    repeat rewrite EPP_subst_iff.
+    intuition.
+
+  * 
+    rewrite EPP_disjoint_iff; auto.
+    2:{ simpl; Actor.simplify. }
+    repeat rewrite EPP_subst_iff.
+    intuition.
+
+  * 
+    rewrite EPP_disjoint_iff; auto.
+    2:{ simpl; Actor.simplify. }
+    repeat rewrite EPP_subst_iff.
+    intuition.
+
+  * 
+    rewrite EPP_disjoint_iff; auto.
+    2:{ simpl; Actor.simplify. }
+    repeat rewrite EPP_subst_iff.
+    intuition.
+    
+  * 
+    apply EPP_cons_iff.
+    intros P. apply IHHstep; auto.
+Qed.
+
+Lemma step_send_EPP : forall C A B PA PB v y refs D PD,
+    EPP A C (Insn.Send v B :: PA) ->
+    EPP B C (Insn.Receive y A :: PB) ->
+    A <> B ->
+    forall C',
+    step_label C refs (Label.Send A v B) C' ->
+
+    EPP D C' PD
+    <->
+    (D = A /\ PD = PA)
+    \/
+    (D = B /\ PD = Process.subst y v PB)
+    \/
+    (D <> A /\ D <> B /\ EPP D C PD).
+Proof.
+  intros C A B PA PB v y refs D PD HA HB Hneq.
+  induction C as [ | I C];
+    intros C' Hstep;
+    simpl in *;
+    inversion Hstep; subst; clear Hstep.
+
+  * (* substitution happens here *)
+    rewrite EPP_subst_iff; auto.
+    inversion HA; subst; clear HA; auto.
+    2:{ (* contradiction *)
+      simpl in *; Actor.simplify.
+    }
+    inversion HB; subst; clear HB; auto.
+    2:{ (* contradiction *)
+      simpl in *; Actor.simplify.
+    }
+    clear H3 H4 H11 H7.
+    split; intros H.
+    + compare D A; [ | compare D B].
+      - left. split; auto.
+        destruct H as [ [PD0 [P0 [HPD0 ?]]] | [? HPD0]]; subst;
+          try contradiction.
+        eapply EPP_deterministic; eauto.
+      - right. left.
+        split; auto.
+        destruct H as [ [PD0 [P0 [HPD0 ?]]] | [? HPD0]]; subst;
+          try contradiction.
+        f_equal.
+        eapply EPP_deterministic; eauto.
+      - right. right.
+        split; auto. split; auto.
+        destruct H as [ [PD0 [P0 [HPD0 ?]]] | [? HPD0]]; subst;
+          try contradiction.
+        constructor; auto.
+        simpl; Actor.simplify.
+
+    + destruct H as [[? ?] | [ [? ?] | [? [? ?]] ]]; subst.
+      - right. split; auto.
+      - left. split; auto. exists PB. split; auto.
+      - right. split; auto.
+        apply EPP_disjoint_inversion in H1; auto.
+        simpl; Actor.simplify.
+
+  * (* substitution happens later *)
+    assert (~ Actor.FSet.In A (Choreography.Insn.actors I)).
+    {
+      intros Hin;
+      match goal with
+      | [ H0 : Actor.FSet.Empty _ |- _ ] => 
+        apply (H0 A)
+      end.
+      simpl; Actor.simplify.
+    }
+    assert (~ Actor.FSet.In B (Choreography.Insn.actors I)).
+    {
+      intros Hin;
+      match goal with
+      | [ H0 : Actor.FSet.Empty _ |- _ ] => 
+        apply (H0 B)
+      end.
+      simpl; Actor.simplify.
+    }
+    clear H1.
+    apply EPP_disjoint_inversion in HA; auto.
+    apply EPP_disjoint_inversion in HB; auto.
+
+    match goal with
+    | [ Hstep0 : step_label C _ _ _ |- _ ] =>
+      set (IH := IHC HA HB _ Hstep0); eauto;
+      rename Hstep0 into Hstep
+    end.
+
+    compare D A; [ | compare D B].
+    - (* D = A *)
+      transitivity (EPP D C'0 PD).
+      { apply EPP_disjoint_iff; auto. }
+      rewrite IH.
+      intuition.
+
+    - (* D = B *)
+      transitivity (EPP D C'0 PD).
+      { apply EPP_disjoint_iff; auto. }
+      rewrite IH.
+      intuition.
+
+    - (* D <> A /\ D <> B *)
+      transitivity (EPP D (I :: C) PD).
+      2:{ intuition. }
+
+      eapply (step_label_neq refs (Label.Send A v B)).
+      2:{ simpl; Actor.simplify. }
+      apply StepCons; auto.
+      { intros Z. simpl. Actor.simplify.
+        intros [[? | ?] Hin']; subst; try contradiction.
+      }
+Qed.
+
+
 
 Lemma subst_neq_inversion : forall A x v D C P,
   D <> A ->
@@ -482,6 +1061,85 @@ Proof.
     destruct (Choreography.Insn.rebound_in A x I) eqn:Hbound;
       auto.
 Qed.
+
+
+Lemma step_send_EPP_N : forall C A B PA PB y v N refs C',
+    EPP_N C N ->
+    EPP A C (Insn.Send v B :: PA) ->
+    EPP B C (Insn.Receive y A :: PB) ->
+    Expr.Val v ->
+    step_label C refs (Label.Send A v B) C' ->
+    EPP_N C' (Actor.Map.add A PA (Actor.Map.add B (Process.subst y v PB) N)).
+Proof.
+  intros C. induction C as [ | I C];
+    intros ? ? ? ? ? ? ? ? ? HN HA HB Hv Hstep.
+  { inversion Hstep. }
+  inversion Hstep; subst; clear Hstep.
+  * (* Case 1: substitution happens here *)
+    inversion HA; subst; clear HA.
+    2:{ simpl in *; Actor.simplify. }
+    inversion HB; subst; clear HB.
+    2:{ simpl in *; Actor.simplify. }
+
+    intros D PD.
+    split; intros H.
+    + Actor.simplify. admit.
+    + Actor.simplify. admit.
+    
+
+  * (* Case 2: substitution happens later *)
+    simpl in *.
+    rename H1 into Hempty; simpl in Hempty.
+    assert (HinA : ~ Actor.FSet.In A (Choreography.Insn.actors I)).
+    { intros H; apply (Hempty A); Actor.simplify. }
+    assert (HinB : ~ Actor.FSet.In B (Choreography.Insn.actors I)).
+    { intros H; apply (Hempty B); Actor.simplify. }
+
+
+  intros D PD. split.
+  * intros Hmaps.
+    Actor.simplify.
+    destruct Hmaps as [[? ?] | Hmaps];
+      subst.
+    + (* D = A *)
+      eapply step_send_complete in Hstep; eauto.
+      inversion Hstep; subst; clear Hstep.
+    inversion HA; subst; clear HA.
+      2:{
+
+      }
+      inversion HB; subst; clear HB.
+Qed.
+
+Lemma step_send_EPP_B : forall C A B PA PB v y,
+    EPP A C (Insn.Send v B :: PA) ->
+    EPP B C (Insn.Receive y A :: PB) ->
+    EPP B (step_send A B C) (Process.subst y v PB).
+Proof.
+  intros C. induction C as [ | I C];
+    intros ? ? ? ? ? ? HA HB;
+    simpl.
+  { inversion HB. }
+
+  inversion HA; subst; clear HA;
+  inversion HB; subst; clear HB;
+    simpl in *; Actor.simplify.
+  { apply EPP_subst_eq; auto. }
+
+  destruct I;
+    try (
+      apply EPP_disjoint; auto;
+      simpl in *; Var.simplify;
+      eapply IHC; eauto;
+        fail
+    ).
+    
+  simpl in *.
+  Actor.simplify.
+  apply EPP_disjoint; simpl; Actor.simplify.
+  eapply IHC; eauto.
+Qed.
+
 
 Lemma step_send_EPP_other : forall C D A B PD,
         D <> A ->
@@ -548,11 +1206,38 @@ Lemma step_send_EPP_N : forall A B C PA PB y v N,
 Proof.
     intros A B C PA PB y v N EPPN EPPA EPPB.
     intros D PD.
-        split; intros HIn.
-    * admit.
-    * destruct HIn as [HIn EPPD].
-      (* Might need a different definition of EPP_N. *)
-Admitted.
+    specialize (EPPN D PD) as EPPN_D.
+    assert (EPP A (step_send A B C) PA).
+    { eapply step_send_EPP_A; eauto. }
+    assert (EPP B (step_send A B C) (Process.subst y v PB)).
+    { eapply step_send_EPP_B; eauto. }
+    split; intros HIn.
+    * Actor.simplify.
+      destruct HIn as [[? ?] | [? [[? HIn] | [? HIn]]]];
+        subst; auto.
+      (* case 3: A <> D /\ B <> D *)
+      eapply step_send_EPP_other; auto.
+      apply EPPN_D; auto.
+
+    * Actor.simplify.
+      compare A D.
+      {
+        Actor.simplify.
+        left. split; auto.
+        eapply EPP_deterministic; eauto.
+      }
+      right. split; auto.
+      compare B D.
+      {
+        left. split; auto.
+        eapply EPP_deterministic; eauto.
+      }
+      right. split; auto.
+      {
+        apply EPPN_D.
+        apply step_send_EPP_other in HIn; auto.
+      }
+Qed.
       
 
 (*
@@ -606,6 +1291,48 @@ Proof.
 Admitted.
 *)
 
+(** Return the choreography C' such that 
+    C -(Local A)-> C'
+*)
+Fixpoint step_local A (C : Choreography.t) : Choreography.t :=
+  match C with
+  | [] => []
+  | Choreography.Insn.Let B x v :: C' =>
+    if Actor.eq_dec A B then Choreography.subst A x v C'
+    else (Choreography.Insn.Let B x v) :: step_local A C'
+  | Choreography.Insn.LetBang B x v :: C' =>
+    if Actor.eq_dec A B
+    then match v with
+         | Expr.Bang v => Choreography.subst A x v C'
+         | _ => []
+         end
+    else (Choreography.Insn.LetBang B x v) :: step_local A C'
+  | Choreography.Insn.LetPair B x1 x2 v :: C' =>
+    if Actor.eq_dec A B
+    then match v with
+         | Expr.Pair v1 v2 => Choreography.subst A x1 v1 (Choreography.subst A x2 v2 C)
+         | _ => []
+         end
+    else (Choreography.Insn.LetPair B x1 x2 v) :: step_local A C'
+  | I0 :: C' => I0 :: step_local A C'
+  end.
+
+Lemma step_let_complete : forall C A x v P,
+    EPP A C (Insn.Let x v :: P) ->
+    Expr.Val v ->
+    forall refs cfg,
+        Choreography.step C refs cfg (Label.Loc A) (step_local A C) refs cfg.
+Proof.
+  induction C as [ | I C]; intros A x v P HEPP Hv refs cfg.
+  { exfalso. inversion HEPP. }
+  inversion HEPP; subst; clear HEPP.
+  * simpl. Actor.simplify.
+    apply Choreography.LetB; auto.
+  * 
+  
+Lemma step_local_not_in :
+  step_local A (I :: C)
+
 
 (** Return the choreography C' such that C, refs, cfg' -(EPR A x B y)-> C' in the configuration cfg *)
 Fixpoint step_epr A B refs cfg (C : Choreography.t) : Choreography.t :=
@@ -657,8 +1384,10 @@ Theorem completeness : forall N refs cfg l N' refs' cfg',
 Proof.
     intros N refs cfg l N' refs' cfg' Hstep.
     induction Hstep; intros C HEPP; subst.
-    
-    * (* local step *) admit.
+  
+    * (* local step *)
+
+
     * (* send *)
       apply HEPP in H0; destruct H0 as [_ HEPPA].
       apply HEPP in H1; destruct H1 as [_ HEPPB].
